Further work on interval splitting

LinearScan/Interval.hs
@@ -102,6 +102,13 @@ firstUseReqReg d =
 
 type IntervalSig = IntervalDesc
 
+splitPosition :: IntervalDesc -> (Prelude.Maybe Prelude.Int) -> Prelude.Int
+splitPosition d before =
+  Lib.fromMaybe
+    (Range.uloc
+      (NonEmpty0.coq_NE_last (Range.ups ( (NonEmpty0.coq_NE_last (rds d))))))
+    (Lib.option_choose before (firstUseReqReg d))
+
 intervalSpan :: (NonEmpty0.NonEmpty Range.RangeSig) -> Prelude.Int ->
                 Prelude.Int -> Prelude.Int ->
                 ((,) (Prelude.Maybe IntervalSig) (Prelude.Maybe IntervalSig))
@@ -109,133 +116,289 @@ intervalSpan rs before ib ie =
   let {f = \u -> (Prelude.<=) (Prelude.succ (Range.uloc u)) before} in
   case rs of {
    NonEmpty0.NE_Sing r ->
-    let {s = Range.rangeSpan f ( r)} in
-    case s of {
-     (,) o o0 ->
-      case o of {
-       Prelude.Just r0 ->
-        case o0 of {
-         Prelude.Just r1 -> (,) (Prelude.Just (Build_IntervalDesc
-          (Range.rbeg ( r0)) (Range.rend ( r0)) (NonEmpty0.NE_Sing ( r0))))
-          (Prelude.Just (Build_IntervalDesc (Range.rbeg ( r1))
-          (Range.rend ( r1)) (NonEmpty0.NE_Sing ( r1))));
-         Prelude.Nothing -> (,) (Prelude.Just (Build_IntervalDesc ib ie
-          (NonEmpty0.NE_Sing r))) Prelude.Nothing};
-       Prelude.Nothing ->
-        case o0 of {
-         Prelude.Just r0 -> (,) Prelude.Nothing (Prelude.Just
-          (Build_IntervalDesc ib ie (NonEmpty0.NE_Sing r)));
-         Prelude.Nothing -> Prelude.error "absurd case"}}};
-   NonEmpty0.NE_Cons r rs0 ->
-    let {s = Range.rangeSpan f ( r)} in
-    case s of {
-     (,) o o0 ->
-      case o of {
-       Prelude.Just r0 ->
-        case o0 of {
-         Prelude.Just r1 ->
-          let {
-           _evar_0_ = \_ ->
-            Ssreflect.ssr_have __ (\_ -> (,) (Prelude.Just
-              (Build_IntervalDesc (Range.rbeg ( r0)) (Range.rend ( r0))
-              (NonEmpty0.NE_Sing ( r0)))) (Prelude.Just (Build_IntervalDesc
-              (Range.rbeg
-                ( (NonEmpty0.coq_NE_head (NonEmpty0.NE_Cons r1 rs0))))
-              (Range.rend ( (NonEmpty0.coq_NE_last rs0))) (NonEmpty0.NE_Cons
-              (NonEmpty0.coq_NE_head (NonEmpty0.NE_Cons r1 rs0)) rs0))))}
-          in
-          Logic.eq_rec_r (Range.rend ( (NonEmpty0.coq_NE_last rs0))) _evar_0_
-            ie __;
-         Prelude.Nothing ->
-          let {
-           _top_assumption_ = intervalSpan rs0 before
-                                (Range.rbeg ( (NonEmpty0.coq_NE_head rs0)))
-                                ie}
-          in
-          let {
-           _evar_0_ = \_top_assumption_0 ->
-            let {
-             _evar_0_ = \o1 _top_assumption_1 ->
-              let {
-               _evar_0_ = \o2 ->
-                let {
-                 _evar_0_ = \_ -> (,) (Prelude.Just (Build_IntervalDesc
-                  (Range.rbeg ( r))
-                  (Range.rend ( (NonEmpty0.coq_NE_last rs0)))
-                  (NonEmpty0.NE_Cons r rs0))) (Prelude.Just o2)}
-                in
-                Logic.eq_rec_r (Range.rend ( (NonEmpty0.coq_NE_last rs0)))
-                  _evar_0_ ie __}
-              in
-              let {
-               _evar_0_0 = \_ ->
-                let {
-                 _evar_0_0 = \_ -> (,) (Prelude.Just (Build_IntervalDesc
-                  (Range.rbeg ( r))
-                  (Range.rend ( (NonEmpty0.coq_NE_last rs0)))
-                  (NonEmpty0.NE_Cons r rs0))) Prelude.Nothing}
-                in
-                Logic.eq_rec_r (Range.rend ( (NonEmpty0.coq_NE_last rs0)))
-                  _evar_0_0 ie __}
-              in
-              case _top_assumption_1 of {
-               Prelude.Just x -> (\_ -> _evar_0_ x);
-               Prelude.Nothing -> _evar_0_0}}
-            in
-            let {
-             _evar_0_0 = \_top_assumption_1 ->
-              let {
-               _evar_0_0 = \o1 -> (,) (Prelude.Just (Build_IntervalDesc ib
-                (Range.rend ( r)) (NonEmpty0.NE_Sing r))) (Prelude.Just
-                (Build_IntervalDesc
-                (Range.rbeg ( (NonEmpty0.coq_NE_head rs0))) ie rs0))}
-              in
-              let {_evar_0_1 = \_ -> (,) Prelude.Nothing Prelude.Nothing} in
-              case _top_assumption_1 of {
-               Prelude.Just x -> (\_ -> _evar_0_0 x);
-               Prelude.Nothing -> _evar_0_1}}
-            in
-            case _top_assumption_0 of {
-             Prelude.Just x -> _evar_0_ x;
-             Prelude.Nothing -> _evar_0_0}}
-          in
-          case _top_assumption_ of {
-           (,) x x0 -> _evar_0_ x x0 __}};
-       Prelude.Nothing ->
-        case o0 of {
-         Prelude.Just r0 -> (,) Prelude.Nothing (Prelude.Just
-          (Build_IntervalDesc ib ie (NonEmpty0.NE_Cons r rs0)));
-         Prelude.Nothing -> Prelude.error "absurd case"}}}}
-
-splitInterval :: Prelude.Int -> IntervalDesc -> ((,) IntervalSig IntervalSig)
-splitInterval before d =
-  let {
-   _evar_0_ = \ibeg0 iend0 rds0 ->
-    let {_top_assumption_ = intervalSpan rds0 before ibeg0 iend0} in
+    let {_top_assumption_ = Range.rangeSpan f ( r)} in
     let {
      _evar_0_ = \_top_assumption_0 ->
       let {
-       _evar_0_ = \o _top_assumption_1 ->
-        let {_evar_0_ = \o0 -> (,) o o0} in
+       _evar_0_ = \r0 _top_assumption_1 ->
+        let {
+         _evar_0_ = \r1 ->
+          let {
+           _evar_0_ = let {
+                       _evar_0_ = \_ _ -> (,) (Prelude.Just
+                        (Build_IntervalDesc (Range.rbeg ( r0))
+                        (Range.rend ( r0)) (NonEmpty0.NE_Sing ( r0))))
+                        (Prelude.Just (Build_IntervalDesc (Range.rbeg ( r1))
+                        (Range.rend ( r1)) (NonEmpty0.NE_Sing ( r1))))}
+                      in
+                      Logic.eq_rec_r (Range.rend ( r1)) _evar_0_
+                        (Range.rend
+                          (Range.getRangeDesc
+                            (
+                              (NonEmpty0.coq_NE_last
+                                (rds (Build_IntervalDesc ib ie
+                                  (NonEmpty0.NE_Sing r)))))))}
+          in
+          Logic.eq_rec_r (Range.rbeg ( r0)) _evar_0_
+            (Range.rbeg
+              (Range.getRangeDesc
+                (
+                  (NonEmpty0.coq_NE_head
+                    (rds (Build_IntervalDesc ib ie (NonEmpty0.NE_Sing r)))))))
+            __ __}
+        in
         let {
          _evar_0_0 = \_ ->
-          let {_evar_0_0 = \_ _ _ -> Logic.coq_False_rec} in
-          Logic.eq_rec (rds (Build_IntervalDesc ibeg0 iend0 rds0)) _evar_0_0
-            (rds ( o)) __}
+          let {
+           _evar_0_0 = \_ -> (,) (Prelude.Just (Build_IntervalDesc ib ie
+            (NonEmpty0.NE_Sing r))) Prelude.Nothing}
+          in
+          Logic.eq_rec (Range.ups ( r)) _evar_0_0 (Range.ups ( r0)) __}
         in
         case _top_assumption_1 of {
-         Prelude.Just x -> (\_ _ _ -> _evar_0_ x);
+         Prelude.Just x -> (\_ -> _evar_0_ x);
          Prelude.Nothing -> _evar_0_0}}
       in
       let {
        _evar_0_0 = \_top_assumption_1 ->
         let {
-         _evar_0_0 = \o0 ->
-          let {_evar_0_0 = \_ _ _ -> Logic.coq_False_rec} in
-          Logic.eq_rec (rds (Build_IntervalDesc ibeg0 iend0 rds0)) _evar_0_0
-            (rds ( o0)) __}
+         _evar_0_0 = \r1 ->
+          let {
+           _evar_0_0 = \_ -> (,) Prelude.Nothing (Prelude.Just
+            (Build_IntervalDesc ib ie (NonEmpty0.NE_Sing r)))}
+          in
+          Logic.eq_rec (Range.ups ( r)) _evar_0_0 (Range.ups ( r1)) __}
         in
-        let {_evar_0_1 = \_ -> Prelude.error "absurd case"} in
+        let {_evar_0_1 = \_ -> Logic.coq_False_rec} in
+        case _top_assumption_1 of {
+         Prelude.Just x -> (\_ -> _evar_0_0 x);
+         Prelude.Nothing -> _evar_0_1}}
+      in
+      case _top_assumption_0 of {
+       Prelude.Just x -> _evar_0_ x;
+       Prelude.Nothing -> _evar_0_0}}
+    in
+    case _top_assumption_ of {
+     (,) x x0 -> _evar_0_ x x0 __};
+   NonEmpty0.NE_Cons r rs0 ->
+    let {_top_assumption_ = Range.rangeSpan f ( r)} in
+    let {
+     _evar_0_ = \_top_assumption_0 ->
+      let {
+       _evar_0_ = \r0 _top_assumption_1 ->
+        let {
+         _evar_0_ = \r1 ->
+          let {
+           _evar_0_ = \_ ->
+            let {
+             _evar_0_ = Ssreflect.ssr_have __ (\_ _ _ -> (,) (Prelude.Just
+                          (Build_IntervalDesc (Range.rbeg ( r0))
+                          (Range.rend ( r0)) (NonEmpty0.NE_Sing ( r0))))
+                          (Prelude.Just (Build_IntervalDesc
+                          (Range.rbeg ( r1))
+                          (Range.rend ( (NonEmpty0.coq_NE_last rs0)))
+                          (NonEmpty0.NE_Cons r1 rs0))))}
+            in
+            Logic.eq_rec_r (Range.rbeg ( r0)) _evar_0_
+              (Range.rbeg
+                (Range.getRangeDesc
+                  (
+                    (NonEmpty0.coq_NE_head
+                      (rds (Build_IntervalDesc ib ie (NonEmpty0.NE_Cons r
+                        rs0))))))) __ __}
+          in
+          Logic.eq_rec_r (Range.rend ( (NonEmpty0.coq_NE_last rs0))) _evar_0_
+            ie __}
+        in
+        let {
+         _evar_0_0 = \_ ->
+          let {
+           _evar_0_0 = \_ ->
+            let {
+             _evar_0_0 = \_ ->
+              let {
+               _top_assumption_2 = intervalSpan rs0 before
+                                     (Range.rbeg
+                                       ( (NonEmpty0.coq_NE_head rs0)))
+                                     (Range.rend
+                                       ( (NonEmpty0.coq_NE_last rs0)))}
+              in
+              let {
+               _evar_0_0 = \_top_assumption_3 ->
+                let {
+                 _evar_0_0 = \i1_1 _top_assumption_4 ->
+                  let {
+                   _evar_0_0 = \i1_2 ->
+                    case i1_1 of {
+                     Build_IntervalDesc ibeg0 iend0 rds0 ->
+                      let {
+                       _evar_0_0 = let {
+                                    _evar_0_0 = \_ ->
+                                     let {
+                                      _evar_0_0 = \_ ->
+                                       let {
+                                        _evar_0_0 = \_ ->
+                                         let {
+                                          _evar_0_0 = Ssreflect.ssr_have __
+                                                        (\_ ->
+                                                        let {
+                                                         _evar_0_0 = \_ _ _ ->
+                                                          (,) (Prelude.Just
+                                                          (Build_IntervalDesc
+                                                          (Range.rbeg ( r))
+                                                          iend0
+                                                          (NonEmpty0.NE_Cons
+                                                          r rds0)))
+                                                          (Prelude.Just
+                                                          i1_2)}
+                                                        in
+                                                        Logic.eq_rec iend0
+                                                          _evar_0_0
+                                                          (Range.rend
+                                                            (
+                                                              (NonEmpty0.coq_NE_last
+                                                                rds0))) __)}
+                                         in
+                                         Logic.eq_rec_r (iend ( i1_2))
+                                           _evar_0_0
+                                           (Range.rend
+                                             (Range.getRangeDesc
+                                               ( (NonEmpty0.coq_NE_last rs0))))}
+                                       in
+                                       Logic.eq_rec_r
+                                         (Range.rbeg
+                                           (Range.getRangeDesc
+                                             ( (NonEmpty0.coq_NE_head rds0))))
+                                         _evar_0_0
+                                         (Range.rbeg
+                                           ( (NonEmpty0.coq_NE_head rs0))) __}
+                                     in
+                                     Logic.eq_rec_r
+                                       (Range.rbeg
+                                         (Range.getRangeDesc
+                                           ( (NonEmpty0.coq_NE_head rds0))))
+                                       _evar_0_0 ibeg0 __}
+                                   in
+                                   Logic.eq_rec_r
+                                     (Range.rend
+                                       (Range.getRangeDesc
+                                         ( (NonEmpty0.coq_NE_last rds0))))
+                                     _evar_0_0 iend0}
+                      in
+                      Logic.eq_rec_r
+                        (Range.rbeg
+                          (Range.getRangeDesc
+                            ( (NonEmpty0.coq_NE_head rds0)))) _evar_0_0 ibeg0
+                        __}}
+                  in
+                  let {
+                   _evar_0_1 = \_ ->
+                    let {
+                     _evar_0_1 = \_ _ _ -> (,) (Prelude.Just
+                      (Build_IntervalDesc (Range.rbeg ( r))
+                      (Range.rend ( (NonEmpty0.coq_NE_last rs0)))
+                      (NonEmpty0.NE_Cons r rs0))) Prelude.Nothing}
+                    in
+                    Logic.eq_rec
+                      (rds (Build_IntervalDesc
+                        (Range.rbeg ( (NonEmpty0.coq_NE_head rs0)))
+                        (Range.rend ( (NonEmpty0.coq_NE_last rs0))) rs0))
+                      _evar_0_1 (rds ( i1_1)) __}
+                  in
+                  case _top_assumption_4 of {
+                   Prelude.Just x -> (\_ -> _evar_0_0 x);
+                   Prelude.Nothing -> _evar_0_1}}
+                in
+                let {
+                 _evar_0_1 = \_top_assumption_4 ->
+                  let {
+                   _evar_0_1 = \i1_2 ->
+                    let {
+                     _evar_0_1 = \_ _ _ -> (,) (Prelude.Just
+                      (Build_IntervalDesc ib (Range.rend ( r))
+                      (NonEmpty0.NE_Sing r))) (Prelude.Just
+                      (Build_IntervalDesc
+                      (Range.rbeg ( (NonEmpty0.coq_NE_head rs0)))
+                      (Range.rend ( (NonEmpty0.coq_NE_last rs0))) rs0))}
+                    in
+                    Logic.eq_rec
+                      (rds (Build_IntervalDesc
+                        (Range.rbeg ( (NonEmpty0.coq_NE_head rs0)))
+                        (Range.rend ( (NonEmpty0.coq_NE_last rs0))) rs0))
+                      _evar_0_1 (rds ( i1_2)) __}
+                  in
+                  let {_evar_0_2 = \_ _ _ -> Logic.coq_False_rec} in
+                  case _top_assumption_4 of {
+                   Prelude.Just x -> (\_ -> _evar_0_1 x);
+                   Prelude.Nothing -> _evar_0_2}}
+                in
+                case _top_assumption_3 of {
+                 Prelude.Just x -> _evar_0_0 x;
+                 Prelude.Nothing -> _evar_0_1}}
+              in
+              case _top_assumption_2 of {
+               (,) x x0 -> _evar_0_0 x x0 __ __ __}}
+            in
+            Logic.eq_rec_r (Range.rend ( (NonEmpty0.coq_NE_last rs0)))
+              _evar_0_0 ie __}
+          in
+          Logic.eq_rec (Range.ups ( r)) _evar_0_0 (Range.ups ( r0)) __}
+        in
+        case _top_assumption_1 of {
+         Prelude.Just x -> (\_ -> _evar_0_ x);
+         Prelude.Nothing -> _evar_0_0}}
+      in
+      let {
+       _evar_0_0 = \_top_assumption_1 ->
+        let {
+         _evar_0_0 = \r1 ->
+          let {
+           _evar_0_0 = \_ -> (,) Prelude.Nothing (Prelude.Just
+            (Build_IntervalDesc ib ie (NonEmpty0.NE_Cons r rs0)))}
+          in
+          Logic.eq_rec (Range.ups ( r)) _evar_0_0 (Range.ups ( r1)) __}
+        in
+        let {_evar_0_1 = \_ -> Logic.coq_False_rec} in
+        case _top_assumption_1 of {
+         Prelude.Just x -> (\_ -> _evar_0_0 x);
+         Prelude.Nothing -> _evar_0_1}}
+      in
+      case _top_assumption_0 of {
+       Prelude.Just x -> _evar_0_ x;
+       Prelude.Nothing -> _evar_0_0}}
+    in
+    case _top_assumption_ of {
+     (,) x x0 -> _evar_0_ x x0 __}}
+
+splitInterval :: Prelude.Int -> IntervalDesc -> ((,) IntervalSig IntervalSig)
+splitInterval before d =
+  let {
+   _evar_0_ = \ib ie rds0 ->
+    let {_top_assumption_ = intervalSpan rds0 before ib ie} in
+    let {
+     _evar_0_ = \_top_assumption_0 ->
+      let {
+       _evar_0_ = \i0 _top_assumption_1 ->
+        let {_evar_0_ = \i1 -> (,) i0 i1} in
+        let {
+         _evar_0_0 = \_ ->
+          let {_evar_0_0 = \_ -> Logic.coq_False_rec} in
+          Logic.eq_rec (rds (Build_IntervalDesc ib ie rds0)) _evar_0_0
+            (rds ( i0)) __}
+        in
+        case _top_assumption_1 of {
+         Prelude.Just x -> (\_ -> _evar_0_ x);
+         Prelude.Nothing -> _evar_0_0}}
+      in
+      let {
+       _evar_0_0 = \_top_assumption_1 ->
+        let {
+         _evar_0_0 = \i1 ->
+          let {_evar_0_0 = \_ -> Logic.coq_False_rec} in
+          Logic.eq_rec (rds (Build_IntervalDesc ib ie rds0)) _evar_0_0
+            (rds ( i1)) __}
+        in
+        let {_evar_0_1 = \_ -> Logic.coq_False_rec} in
         case _top_assumption_1 of {
          Prelude.Just x -> (\_ -> _evar_0_0 x);
          Prelude.Nothing -> _evar_0_1}}
@@ -248,5 +411,5 @@ splitInterval before d =
      (,) x x0 -> _evar_0_ x x0 __}}
   in
   case d of {
-   Build_IntervalDesc x x0 x1 -> _evar_0_ x x0 x1 __ __}
+   Build_IntervalDesc x x0 x1 -> _evar_0_ x x0 x1}
 
