Vector.v
@@ -33,8 +33,8 @@ Definition relocate {A n} (v : Vec A n) (p q : fin n) : Vec A n :=
 Definition modify {A n} (v : Vec A n) (p : fin n) (f : A -> A) : Vec A n :=
   V.replace v (to_vfin p) (f (V.nth v (to_vfin p))).
 
-Definition fold_left_with_index {A B : Type} {n} (f : fin n -> B -> A -> B)
-  : forall (b : B) (v : Vec A n), B.
+Definition fold_left_with_index {A B : Type} {n} (f : fin n -> B -> A -> B) :
+  forall (b : B) (v : Vec A n), B.
   intros b v.
   induction v.
     apply b.
